proof/invariant-abstract/Tcb_AI.thy
@@ -123,14 +123,6 @@ lemma (in Tcb_AI_1) activate_invs:
   apply (wpsimp wp: complete_yield_to_invs)
   done
 
-lemma cancel_ipc_no_refs:
-  "\<lbrace>\<lambda>s. sym_refs (state_refs_of s) \<and> valid_objs s\<rbrace>
-  cancel_ipc t \<lbrace>\<lambda>_. st_tcb_at (\<lambda>st'. tcb_st_refs_of st' = {}) t\<rbrace>"
-  apply (rule hoare_strengthen_post)
-   apply (rule cancel_ipc_simple_except_awaiting_reply)
-  apply (auto elim: st_tcb_weakenE)
-  done
-
 crunch test_possible_switch_to
  for invs[wp]: invs
 
@@ -330,7 +322,7 @@ lemma tcb_sched_action_valid_tcb[wp]:
 
 lemma set_thread_state_valid_tcb[wp]:
   "\<lbrace>valid_tcb ptr tcb and valid_tcb_state st\<rbrace> set_thread_state thread st \<lbrace>\<lambda>_. valid_tcb ptr tcb\<rbrace>"
-  apply (clarsimp simp: set_thread_state_def set_thread_state_act_def)
+  apply (clarsimp simp: set_thread_state_def thread_set_def set_thread_state_act_def)
   apply (rule bind_wp_fwd_skip, wpsimp)
   apply (rule_tac Q'="\<lambda>_. valid_tcb ptr tcb" in bind_wp_fwd)
    apply (wpsimp wp: set_object_valid_tcbs)
@@ -341,7 +333,7 @@ lemma set_thread_state_valid_tcb[wp]:
 
 lemma set_thread_state_valid_tcbs[wp]:
   "\<lbrace>valid_tcbs and valid_tcb_state st\<rbrace> set_thread_state thread st \<lbrace>\<lambda>_. valid_tcbs\<rbrace>"
-  apply (clarsimp simp: set_thread_state_def set_thread_state_act_def)
+  apply (clarsimp simp: set_thread_state_def thread_set_def set_thread_state_act_def bind_assoc)
   apply (rule bind_wp[OF _ gets_the_get_tcb_sp])
   apply (rule_tac Q'="\<lambda>_. valid_tcbs" in bind_wp_fwd)
    apply (wpsimp wp: set_object_valid_tcbs)
@@ -1723,11 +1715,11 @@ lemma set_notification_obj_at_impossible:
 
 lemma reorder_ntfn_sc_tcb_sc_at[wp]:
   "reorder_ntfn ntfn_ptr tptr \<lbrace>\<lambda>s. Q (sc_tcb_sc_at P t s)\<rbrace>"
-  by (wpsimp wp: get_simple_ko_wp simp: reorder_ntfn_def)
+  by (wpsimp wp: get_simple_ko_wp simp: reorder_ntfn_def get_ntfn_queue_def)
 
 lemma reorder_ep_sc_tcb_sc_at[wp]:
   "reorder_ep ntfn_ptr tptr \<lbrace>\<lambda>s. Q (sc_tcb_sc_at P t s)\<rbrace>"
-  by (wpsimp wp: get_simple_ko_wp simp: reorder_ntfn_def reorder_ep_def)
+  by (wpsimp wp: get_simple_ko_wp simp: reorder_ntfn_def reorder_ep_def get_ep_queue_def)
 
 lemma thread_set_priority_ex_nonz_cap_to[wp]:
   "thread_set_priority t p \<lbrace>ex_nonz_cap_to p'\<rbrace>"
@@ -1772,36 +1764,34 @@ lemma inj_on_snd_set_zip_map:
   "distinct xs \<Longrightarrow> inj_on snd (set (zip (map f xs) xs))"
   using distinct_map by fastforce
 
-lemma tcb_ep_dequeue_append_valid_ntfn_rv:
+lemma ordered_insert_singleton[wp]:
+  "\<lbrace>\<lambda>s. ts = [] \<and> tcb_ptr = t\<rbrace> ordered_insert t ts f R \<lbrace>\<lambda>ts' _. ts' = [tcb_ptr]\<rbrace>"
+  unfolding ordered_insert_def
+  by (wpsimp wp: mapM_gets_the_wp')
+
+lemma tcb_dequeue_append_valid_ntfn_rv:
   "\<lbrace>valid_ntfn ntfn and K (ntfn_obj ntfn = WaitingNtfn qs \<and> t \<in> set qs)\<rbrace>
-   do qs' \<leftarrow> tcb_ep_dequeue t qs;
-      tcb_ep_append t qs'
+   do qs' \<leftarrow> tcb_dequeue t qs;
+      tcb_append t qs'
    od
    \<lbrace>\<lambda>rv s. valid_ntfn (ntfn_set_obj ntfn (WaitingNtfn rv)) s\<rbrace>"
-  apply (rule hoare_weaken_pre)
-   apply (rule monadic_rewrite_refine_valid)
-     apply (rule monadic_rewrite_bind_tail)
-      apply (rule monadic_rewrite_sym)
-      apply (rule tcb_ep_append_insort_filter)
-     apply (wpsimp simp: tcb_ep_append_def tcb_ep_dequeue_def)
-    apply (clarsimp simp: valid_ntfn_def split: option.split)
-    apply (simp add: tcb_ep_append_def tcb_ep_dequeue_def)
-    apply wpsimp
-   apply fastforce
-  apply (fastforce simp: valid_ntfn_def insort_filter_def distinct_insort_filter
-                  split: option.splits)
+  unfolding valid_ntfn_def
+  apply (clarsimp simp: tcb_dequeue_def tcb_append_def)
+  apply (wpsimp wp: hoare_case_option_wp2)
+  apply (clarsimp split: option.splits)
   done
 
 lemma reorder_ntfn_invs[wp]:
-  "\<lbrace>invs and st_tcb_at (\<lambda>st. ntfn_blocked st = Some nptr) tptr\<rbrace> reorder_ntfn nptr tptr \<lbrace>\<lambda>rv. invs\<rbrace>"
-  apply (simp only: reorder_ntfn_def)
-  apply (subst bind_assoc[symmetric, where m="tcb_ep_dequeue tptr _"])
+  "\<lbrace>invs and st_tcb_at (\<lambda>st. ntfn_blocked st = Some nptr) tptr\<rbrace> reorder_ntfn nptr tptr \<lbrace>\<lambda>_. invs\<rbrace>"
+  apply (simp add: reorder_ntfn_def get_ntfn_queue_def)
+  apply (rule bind_wp[OF _ get_simple_ko_sp])
+  apply (subst bind_assoc[symmetric, where m="tcb_dequeue tptr _"])
   apply (rule bind_wp)+
      \<comment> \<open>tcb_ep_dequeue_append_valid_ntfn_rv requires that the postcondition conjunctions are
         carefully managed, so that the bind is not split too early\<close>
-     apply (wpsimp wp: set_ntfn_minor_invs get_simple_ko_wp tcb_ep_dequeue_rv_wf'
-                       tcb_ep_dequeue_append_valid_ntfn_rv hoare_elim_pred_conj
-                 simp: live_def live_ntfn_def pred_conj_def)+
+   apply (wpsimp wp: set_ntfn_minor_invs get_simple_ko_wp tcb_dequeue_rv_wf'
+                     tcb_dequeue_append_valid_ntfn_rv hoare_elim_pred_conj
+               simp: live_def live_ntfn_def pred_conj_def)+
   apply (frule valid_objs_ko_at[rotated], fastforce)
   apply (clarsimp simp: valid_obj_def valid_ntfn_def obj_at_def pred_tcb_at_def cong: conj_cong)
   apply (case_tac "tcb_state tcb"; clarsimp simp: ntfn_blocked_def get_ntfn_queue_def split: ntfn.splits)
@@ -1834,12 +1824,12 @@ lemma set_ep_minor_invs:
   done
 
 lemma reorder_ep_invs[wp]:
-  "\<lbrace>invs and st_tcb_at (\<lambda>st. ep_blocked st = Some nptr) tptr\<rbrace> reorder_ep nptr tptr \<lbrace>\<lambda>rv. invs\<rbrace>"
+  "\<lbrace>invs and st_tcb_at (\<lambda>st. ep_blocked st = Some nptr) tptr\<rbrace> reorder_ep nptr tptr \<lbrace>\<lambda>_. invs\<rbrace>"
   apply (simp only: reorder_ep_def get_ep_queue_def endpoint.case_eq_if if_cancel)
   apply (rule bind_wp[OF _ get_simple_ko_sp])
-  apply (wp set_ep_minor_invs hoare_drop_imps tcb_ep_dequeue_rv_wf'
-            tcb_ep_dequeue_valid_ep tcb_ep_dequeue_inv tcb_ep_dequeue_rv_wf''
-            tcb_ep_append_valid_ep tcb_ep_append_inv tcb_ep_append_rv_wf''')
+  apply (wp set_ep_minor_invs hoare_drop_imps tcb_dequeue_rv_wf'
+            tcb_dequeue_valid_ep tcb_dequeue_inv tcb_dequeue_rv_wf''
+            tcb_append_valid_ep tcb_append_inv tcb_append_rv_wf''')
   apply (clarsimp cong: conj_cong)
   apply (rename_tac ep s)
   apply (frule valid_objs_ko_at[rotated], fastforce)
